Revert Expr changes; verified quasi-reasonable malloc() with some nasty non-automation and one 'obvious' admitted fact about bitvectors

examples/Malloc.v
@@ -1,5 +1,5 @@
 Require Import AutoSep.
-Require Import List.
+Require Import Arith List.
 
 Set Implicit Arguments.
 
@@ -74,6 +74,22 @@ Qed.
 
 Hint Extern 1 (himp _ (allocated _ _ _) (allocated _ _ _)) => apply allocated_shift_base.
 
+Theorem allocated_split : forall base len' len offset,
+  (len' <= len)%nat
+  -> allocated base offset len ===> allocated base offset len' * allocated base (offset + 4 * len') (len - len').
+  induction len'; simpl; inversion 1; sepLemma.
+  rewrite plus_0_r; sepLemma.
+  rewrite minus_diag; sepLemma.
+  specialize (IHlen' m (S (S (S (S offset))))).
+  assert (len' <= m)%nat by omega.
+  intuition.
+  match goal with
+    | [ _ : _ ===> _ * allocated _ ?X _ |- himp _ _ (SEP.ST.star _ (allocated _ ?Y _)) ] =>
+      replace Y with X by omega
+  end.
+  auto.
+Qed.
+  
 
 (** * A free-list heap managed by the malloc library *)
 
@@ -89,13 +105,13 @@ Module Type FREE_LIST.
 
   Axiom nil_bwd : forall n p, p = 0 -> [| n = 0 |] ===> freeList n p.
   Axiom cons_bwd : forall n (p : W), p <> 0
-    -> (Ex n', Ex sz, Ex p', [| n = S n' /\ goodSize sz |] * (p ==*> $(sz), p')
+    -> (Ex n', Ex sz, Ex p', [| n = S n' /\ goodSize (sz+2) |] * (p ==*> $(sz), p')
       * (p ^+ $8) =?> sz * freeList n' p')
     ===> freeList n p.
 
   Axiom cons_fwd : forall n (p : W), p <> 0
     -> freeList n p
-    ===> Ex n', Ex sz, Ex p', [| n = S n' /\ goodSize sz |] * (p ==*> $(sz), p')
+    ===> Ex n', Ex sz, Ex p', [| n = S n' /\ goodSize (sz+2) |] * (p ==*> $(sz), p')
     * (p ^+ $8) =?> sz * freeList n' p'.
 End FREE_LIST.
 
@@ -105,7 +121,7 @@ Module FreeList : FREE_LIST.
   Fixpoint freeList (n : nat) (p : W) : HProp :=
     match n with
       | O => [| p = 0 |]
-      | S n' => [| p <> 0 |] * Ex sz, Ex p', [| goodSize sz |] * (p ==*> $(sz), p')
+      | S n' => [| p <> 0 |] * Ex sz, Ex p', [| goodSize (sz+2) |] * (p ==*> $(sz), p')
         * (p ^+ $8) =?> sz * freeList n' p'
     end.
 
@@ -132,7 +148,7 @@ Module FreeList : FREE_LIST.
   Qed.
 
   Theorem cons_bwd : forall n (p : W), p <> 0
-    -> (Ex n', Ex sz, Ex p', [| n = S n' /\ goodSize sz |] * (p ==*> $(sz), p')
+    -> (Ex n', Ex sz, Ex p', [| n = S n' /\ goodSize (sz+2) |] * (p ==*> $(sz), p')
       * (p ^+ $8) =?> sz * freeList n' p')
     ===> freeList n p.
     destruct n; sepLemma; match goal with
@@ -142,7 +158,7 @@ Module FreeList : FREE_LIST.
 
   Theorem cons_fwd : forall n (p : W), p <> 0
     -> freeList n p
-    ===> Ex n', Ex sz, Ex p', [| n = S n' /\ goodSize sz |] * (p ==*> $(sz), p')
+    ===> Ex n', Ex sz, Ex p', [| n = S n' /\ goodSize (sz+2) |] * (p ==*> $(sz), p')
     * (p ^+ $8) =?> sz * freeList n' p'.
     destruct n; sepLemma.
   Qed.
@@ -152,23 +168,138 @@ Import FreeList.
 Export FreeList.
 Hint Immediate freeList_extensional mallocHeap_extensional.
 
+Lemma wordToNat_natToWord_idempotent : forall sz n,
+  (N.of_nat n < Npow2 sz)%N
+  -> wordToNat (natToWord sz n) = n.
+  intros.
+  destruct (wordToNat_natToWord sz n); intuition.
+  destruct x.
+  simpl in *; omega.
+  simpl in *.
+  apply Nlt_out in H.
+  autorewrite with N in *.
+  rewrite Npow2_nat in *.
+  generalize dependent (x * pow2 sz).
+  intros; omega.
+Qed.
+
+Lemma wplus_lt_lift : forall sz n m o : nat,
+  (N.of_nat (n + m) < Npow2 sz)%N
+  -> (N.of_nat o < Npow2 sz)%N
+  -> natToWord sz n ^+ natToWord sz m < natToWord sz o
+  -> (n + m < o)%nat.
+  unfold wlt; intros.
+  rewrite wplus_alt in *.
+  unfold wplusN, wordBinN in *.
+  repeat rewrite wordToNat_natToWord_idempotent in * by nomega.
+  repeat rewrite wordToN_nat in *.
+  repeat rewrite wordToNat_natToWord_idempotent in * by nomega.
+  nomega.
+Qed.
+
+Lemma goodSize_plus_l : forall n m sz, (N.of_nat (n + m) < sz)%N -> (N.of_nat n < sz)%N.
+  unfold goodSize; intros; nomega.
+Qed.
+
+Lemma malloc_split' : forall cur full init,
+  (init < full)%nat
+  -> cur =?> full ===> cur =?> init * allocated cur (init * 4) (full - init).
+  intros.
+  replace (init * 4) with (4 * init) by omega.
+  assert (Hle : (init <= full)%nat) by omega.
+  apply (@allocated_split cur init full 0 Hle).
+Qed.
+
+Lemma Himp_trans : forall p q r,
+  p ===> q
+  -> q ===> r
+  -> p ===> r.
+  unfold Himp, himp; eauto using Imply_trans.
+Qed.
+
+Lemma natToWord_times4 : forall n, natToW (n * 4) = natToW n ^* natToW 4.
+  intros.
+  replace (natToW n ^* natToW 4) with (natToW n ^+ (natToW n ^+ (natToW n ^+ (natToW n ^+ natToW 0)))).
+  autorewrite with sepFormula.
+  intros; rewrite mult_comm; simpl.
+  reflexivity.
+  W_eq.
+Qed.
+
+Hint Rewrite natToWord_times4 : sepFormula.
+
+Definition splitMe cur full (_ : nat) := (cur =?> full)%Sep.
+
+Section malloc_split.
+  Hint Immediate goodSize_plus_l.
+  Hint Resolve wplus_lt_lift.
+
+  Lemma malloc_split'' : forall cur full init,
+    goodSize (init + 2)
+    -> goodSize (full + 2)
+    -> natToW init ^+ natToW 2 < natToW full
+    -> splitMe cur full init ===> cur =?> (full - init - 2) * allocated cur ((full - (init + 2)) * 4) (init + 2).
+    intros.
+    replace (full - init - 2) with (full - (init + 2)) by omega.
+    replace (allocated cur ((full - (init + 2)) * 4) (init + 2))
+      with (allocated cur ((full - (init + 2)) * 4) (full - (full - (init + 2)))).
+    apply malloc_split'; eauto.
+    apply wplus_lt_lift in H1.
+    omega.
+    auto.
+    eauto.
+    f_equal.
+    apply wplus_lt_lift in H1.
+    omega.
+    auto.
+    eauto.
+  Qed.
+
+  Lemma malloc_split''' : forall cur full init,
+    goodSize (init + 2)
+    -> goodSize (full + 2)
+    -> natToW init ^+ natToW 2 < natToW full
+    -> splitMe cur full init ===> cur =?> (full - init - 2) * (cur ^+ $ ((full - (init + 2)) * 4)%nat) =?> (init + 2).
+    intros; eapply Himp_trans.
+    apply malloc_split''; auto.
+    sepLemma.
+    apply allocated_shift_base; auto.
+    autorewrite with sepFormula.
+    W_eq.
+  Qed.
+
+  Lemma malloc_split : forall cur full init,
+    goodSize (init + 2)
+    -> goodSize (full + 2)
+    -> natToW init ^+ natToW 2 < natToW full
+    -> splitMe cur full init ===> cur =?> (full - init - 2)
+    * (Ex v, (cur ^+ $ ((full - (init + 2)) * 4)%nat) =*> v)
+    * (Ex v, (cur ^+ $ ((full - (init + 2)) * 4) ^+ $4) =*> v)
+    * allocated (cur ^+ $ ((full - (init + 2)) * 4)) 8 init.
+    intros; eapply Himp_trans.
+    apply malloc_split'''; auto.
+    rewrite plus_comm; simpl.
+    sepLemma.
+  Qed.
+End malloc_split.
+
 Definition hints' : TacPackage.
-  prepare1 (mallocHeap_fwd, cons_fwd) (mallocHeap_bwd, nil_bwd, cons_bwd).
+  prepare1 (mallocHeap_fwd, cons_fwd, malloc_split) (mallocHeap_bwd, nil_bwd, cons_bwd).
 Defined.
 
 Definition hints : TacPackage.
   prepare2 hints'.
 Defined.
 
-Definition initS : assert := st ~> ExX, Ex n, [| st#Rv = $(n) /\ goodSize n |]
+Definition initS : assert := st ~> ExX, Ex n, [| st#Rv = $(n) /\ goodSize (n+2) |]
   /\ ![ ^[0 =?> (3 + n)] * #0 ] st
   /\ st#Rp @@ (st' ~> [| st'#Sp = st#Sp |] /\ ![ ^[mallocHeap] * #1 ] st').
 
-Definition freeS : assert := st ~> ExX, Ex p : W, Ex n, [| p <> 0 /\ goodSize n |]
+Definition freeS : assert := st ~> ExX, Ex p : W, Ex n, [| p <> 0 /\ goodSize (n+2) |]
   /\ ![ (st#Sp ==*> p, $(n)) * ^[p =?> (2 + n)] * ^[mallocHeap] * #0 ] st
   /\ st#Rp @@ (st' ~> [| st'#Sp = st#Sp |] /\ ![ (st#Sp ==*> p, $(n)) * ^[mallocHeap] * #1 ] st').
 
-Definition mallocS : assert := st ~> ExX, Ex sz, Ex v, [| goodSize sz |]
+Definition mallocS : assert := st ~> ExX, Ex sz, Ex v, [| goodSize (sz+2) |]
   /\ ![ (st#Sp ==*> $(sz), v) * ^[mallocHeap] * #0 ] st
   /\ st#Rp @@ (st' ~> [| st'#Sp = st#Sp |]
     /\ Ex a, Ex b, ![ (st#Sp ==*> a, b) * ^[st'#Rv =?> (2 + sz)] * ^[mallocHeap] * #1 ] st').
@@ -190,7 +321,7 @@ Definition mallocM := bmodule "malloc" {{
     $[Sp+4] <- Rp;;
     Rp <- 0;;
 
-    [st ~> ExX, Ex sz, Ex ret, Ex n, [| goodSize sz |]
+    [st ~> ExX, Ex sz, Ex ret, Ex n, [| goodSize (sz+2) |]
       /\ ![ (st#Sp ==*> $(sz), ret) * st#Rp =*> st#Rv * ^[freeList n st#Rv] * #0 ] st
       /\ ret @@ (st' ~> [| st'#Sp = st#Sp |]
         /\ Ex a, Ex b, Ex n', Ex p,
@@ -206,11 +337,19 @@ Definition mallocM := bmodule "malloc" {{
         Rp <- $[Sp] + 2;;
         If (Rp < $[Rv]) {
           (* This free list block is large enough to split in two. *)
-          Rp <- Rv + $[Sp];;
-          Rp <- Rp + 2;;
-          $[Rp] <- $[Rv] - $[Sp];;
-          $[Rp] <- $[Rp] - 2;;
-          $[Rp+4] <- $[Rv+4];;
+
+          (* Calculate starting address of a suffix of this free block to return to caller. *)
+          Rp <- $[Rv] - $[Sp];;
+          Rp <- 4 * Rp;;
+          Rp <- Rv + Rp;;
+
+          (* Decrement size of free list block to reflect deleted suffix. *)
+          $[Rv] <- $[Rv] - $[Sp];;
+          $[Rv] <- $[Rv] - 2;;
+
+          (* Return suffix starting address. *)
+          Rv <- Rp;;
+          Rp <- $[Sp+4];;
           Return Rv
         } else {
           (* Current block too small; continue to next. *)
@@ -234,7 +373,42 @@ Hint Extern 2 (@eq (word _) _ _) =>
     | [ H : _ = _ |- _ ] => rewrite <- H; W_eq
   end.
 
-Hint Immediate natToW_inj.
+Hint Resolve natToW_inj.
+
+Lemma natToWord_minus : forall sz n m, (m <= n)%nat
+  -> natToWord sz (n - m) = natToWord _ n ^- natToWord _ m.
+Admitted.
+
+Lemma natToW_minus : forall n m, (m <= n)%nat
+  -> natToW (n - m) = natToW n ^- natToW m.
+  intros; apply natToWord_minus; auto.
+Qed.
+
+Lemma cancel8 : forall x y z,
+  (z + 2 <= y)%nat
+  -> x ^+ $8 ^+ $((y - (z + 2)) * 4) = x ^+ $4 ^* ($(y) ^- natToW z).
+  intros.
+  autorewrite with sepFormula.
+  rewrite natToW_minus by auto.
+  rewrite natToW_plus.
+  unfold natToW.
+  W_eq.
+Qed.
+
+Lemma goodSize_p2 : forall n,
+  goodSize (n + 2)
+  -> goodSize n.
+  intros; eapply goodSize_plus_l; eauto.
+Qed.
+
+Lemma goodSize_diff : forall x y z,
+  (N.of_nat (x + 2) < z)%N
+  -> (N.of_nat (x - y - 2 + 2) < z)%N.
+  intros; nomega.
+Qed.
+
+Hint Immediate goodSize_p2.
+Hint Extern 1 (goodSize (_ - _ - _ + _ )) => apply goodSize_diff.
 
 Theorem mallocMOk : moduleOk mallocM.
   vcgen.
@@ -254,8 +428,39 @@ Theorem mallocMOk : moduleOk mallocM.
   t.
   t.
   t.
-  admit.
-  admit.
+  t.
+
+  evaluate hints.
+  match goal with
+    | [ _ : natToW ?init ^+ natToW 2 < natToW ?full,
+        H : context[(?base =?> ?full)%Sep] |- _ ] =>
+      change (base =?> full)%Sep with (splitMe base full init) in H
+  end.
+  evaluate hints.
+  descend.
+  step hints.
+  step hints.
+  descend.
+  step hints.
+  step hints.
+  auto.
+  rewrite cancel8.
+  step hints.
+  repeat rewrite natToW_minus.
+  step hints.
+  apply wplus_lt_lift in H32; auto.
+  omega.
+  eapply goodSize_plus_l; eauto.
+  apply wplus_lt_lift in H32; auto.
+  omega.
+  eauto.
+  eapply goodSize_plus_l; eauto.
+  apply wplus_lt_lift in H32; auto.
+  omega.
+  apply wplus_lt_lift in H32; auto.
+  eapply goodSize_plus_l; eauto.
+  eapply goodSize_plus_l; eauto.
+
   t.
 
   (*vcgen; abstract (pose four_neq_zero; sep hints; auto).*)
